clean closed subst / inversion

process/substitution.v
@@ -1,148 +1,495 @@
 From mathcomp Require Import all_ssreflect.
-From SST Require Import aux.unscoped aux.expressions process.processes process.typecheck process.inversion type.global tree.global tree.local.
+From SST Require Import aux.unscoped aux.expressions process.processes process.typecheck process.inversion process.inversion_expr type.global tree.global tree.local.
 Require Import List String Datatypes ZArith Relations PeanoNat.
 Open Scope list_scope.
 From mathcomp Require Import ssreflect.seq.
 Import ListNotations.
 From Paco Require Import paco.
 
-Lemma _typ_consistency_ : forall em Gs Gt P T, typ_proc em Gs Gt P T -> (consistent_ctxS Gs /\ consistent_ctxT Gt).
+
+Fixpoint RemoveT (n : fin) (Gt : ctxT) : ctxT :=
+  match Gt with 
+    | x::xs =>
+      match n with 
+        | S m => x :: RemoveT m xs
+        | 0   => None :: xs 
+      end
+    | [] => []
+  end.
+
+Fixpoint extendT (n : fin) (T : ltt) (Gt : ctxT) : ctxT :=
+  match Gt with 
+    | x::xs =>
+      match n with 
+        | S m => x :: extendT m T xs
+        | 0   => Some T :: xs 
+      end 
+    | [] =>
+      match n with 
+        | S m => None :: extendT m T [] 
+        | 0   => [Some T]
+      end 
+  end.
+  
+Lemma onth_nil : forall n, @onth ltt n [] = None.
 Proof.
-intros.
-  induction H using typ_proc_ind_ref; intros; try easy.
-  destruct IHtyp_proc.
-  split; try easy. simpl in H1. destruct H1. easy. 
-  destruct H2. 
-  - simpl in H. specialize(eq_trans H H0); intros. specialize(eq_trans H2 H1); intros. clear H0 H1.
-    specialize(positive_list_length_dst ST 0 (eq_sym H)); intros.
-    specialize(positive_list_length_dst Pr 0 (eq_sym H2)); intros.
-    specialize(positive_list_length_dst T 0 (eq_sym H4)); intros.
-    destruct H0. destruct H0. destruct H1. destruct H1. destruct H5. destruct H5. subst.
-    specialize(Forall2_cons_iff (fun (_ : process) (v : sort * ltt) =>
-        consistent_ctxS (extendS cs em (fst v)) /\ consistent_ctxT ct) x1 (x,x3) x2 (zip x0 x4)); intros.
-    destruct H0. clear H1. specialize(H0 H3); intros. clear H3. destruct H0. destruct H0. 
-    simpl in H0. destruct H0. easy.
-  - simpl in H. specialize(eq_trans H H0); intros. specialize(eq_trans H5 H1); intros. clear H0 H1.
-    specialize(positive_list_length_dst ST (S (length l)) (eq_sym H)); intros.
-    specialize(positive_list_length_dst Pr (S (length l)) (eq_sym H5)); intros.
-    specialize(positive_list_length_dst T (S (length l)) (eq_sym H6)); intros.
-    destruct H0. destruct H0. destruct H1. destruct H1. destruct H7. destruct H7. subst.
-    specialize(Forall2_cons_iff (fun (_ : process) (v : sort * ltt) =>
-        consistent_ctxS (extendS cs em (fst v)) /\ consistent_ctxT ct) x1 (x,x3) x2 (zip x0 x4)); intros.
-    destruct H0. clear H1. specialize(H0 H3); intros. clear H3. destruct H0. destruct H0. 
-    simpl in H0. destruct H0. easy.    
+  intros. induction n. easy. easy.
 Qed.
 
-Lemma trivial_type_inact : forall em Gs Gt T, typ_proc em Gs Gt p_inact T -> T = ltt_end.
+Lemma remove_var : forall X n T Gt x, X <> n -> onth n (extendT X T Gt) = Some x -> onth n Gt = Some x.
+Proof.
+  intros X n T Gt. revert X T Gt. induction n; intros; try easy.
+  destruct X; try easy. destruct Gt. easy. simpl in H0. simpl. easy.
+  destruct X. destruct Gt; try easy. simpl in H0. simpl. 
+  specialize(onth_nil n); intros.
+  specialize(eq_trans (ssrfun.esym H1) H0); intros. easy.
+  specialize(Nat.succ_inj_wd_neg X n); intros. destruct H1. 
+  specialize(H1 H); intros. clear H2.
+  destruct Gt. 
+  - simpl in H0.
+    specialize(IHn X T [] x H1 H0); intros.
+    specialize(onth_nil n); intros.
+    specialize(eq_trans (ssrfun.esym H2) IHn); intros. easy.
+  - simpl in *. 
+    apply IHn with (X := X) (T := T); try easy.
+Qed.
+
+Lemma extend_extract : forall n (T : ltt) Gt, onth n (extendT n T Gt) = Some T.
+Proof.
+  intro n. induction n using strong_ind.
+  intros t gt. revert t. induction gt.
+  - intros. destruct n. easy.
+    simpl. apply H; try easy. apply Nat.lt_succ_diag_r.
+  - intros. destruct n. easy.
+    simpl. apply H; try easy. apply Nat.lt_succ_diag_r.
+Qed.
+
+Lemma positive_list_length_dst {A} : forall (xs : list A) n, length xs = S(n) -> exists y ys, y::ys = xs.
+Proof.
+  intros.
+  induction xs. easy.
+  exists a. exists xs. easy.
+Qed.
+
+Lemma positive_list_length_dst_zip {A B} : forall (xs : list A) (ys : list B) n, length (zip xs ys) = S n -> exists t ts u us, (t,u) :: zip ts us = zip xs ys.
 Proof.
   intros. 
-  specialize(_a23_f p_inact em T Gs Gt H (eq_refl p_inact)); intros.
-  easy.
+  specialize(positive_list_length_dst (zip xs ys) n H); intros.
+  destruct H0. destruct H0.
+  exists x.1. exists (list_map fst x0). exists x.2. exists (list_map snd x0).
+  specialize(unzip_zip x0); intros. 
+  replace (zip (list_map fst x0) (list_map snd x0)) with x0.
+  specialize(surjective_pairing x); intros. 
+  replace (x.1, x.2) with x. easy.
 Qed.
 
-Lemma remove_unusedT_inact : forall em Gs Gt X T T',
-  typ_proc em Gs (extendT Gt X T) p_inact T' -> typ_proc em Gs Gt p_inact T'.
+Lemma slideT_helper : forall llp x0 x X m k l Gs Gtl Gtr tm,
+    Forall
+      (fun Q : process =>
+       forall (X m l k : fin) (tm : option ltt) (Gs : ctxS) (Gtl Gtr : seq (option ltt))
+         (T : ltt),
+       typ_proc Gs (Gtl ++ Gtr) (incr_free l k X m Q) T ->
+       length Gtl = l -> typ_proc Gs (Gtl ++ tm :: Gtr) (incr_free l k X.+1 m Q) T) llp ->
+    Forall2 (fun (u : process) (v : sort * ltt) => typ_proc (Some v.1 :: Gs) (Gtl ++ Gtr) u v.2)
+       (list_map (incr_free l k.+1 X m) llp) (zip x0 x) ->
+    length Gtl = l ->
+    Forall2
+      (fun (u : process) (v : sort * ltt) => typ_proc (Some v.1 :: Gs) (Gtl ++ tm :: Gtr) u v.2)
+      (list_map (incr_free l k.+1 X.+1 m) llp) (zip x0 x).
+Proof.
+  intro llp. induction llp; intros; try easy.
+  - specialize(Forall2_length H0); intros.
+    specialize(map_length (incr_free 0 1 X m) []); intros.
+    specialize(eq_trans (esym H2) H3); intros. simpl in H4.
+    specialize(length_zero_iff_nil (zip x0 x)); intros. destruct H5. specialize(H5 H4); intros.
+    replace (zip x0 x) with (@nil (sort * ltt)). easy.
+  - specialize(Forall2_length H0); intros.
+    specialize(map_length (incr_free l k.+1 X m) (a::llp)); intros.
+    specialize(eq_trans (esym H2) H3); intros. simpl in H4.
+    specialize(positive_list_length_dst_zip x0 x (length llp) H4); intros.
+    destruct H5. destruct H5. destruct H5. destruct H5. 
+    replace (zip x0 x) with ((x1,x3) :: zip x2 x4) in *. clear H2 H3 H4 H5.
+    simpl in H0.
+    specialize(Forall2_cons_iff (fun (u : process) (v : sort * ltt) => typ_proc (Some v.1 :: Gs) (Gtl ++ Gtr) u v.2) (incr_free l k.+1 X m a) (x1,x3) (list_map (incr_free l k.+1 X m) llp) (zip x2 x4)); intros.
+    destruct H2. clear H3. specialize(H2 H0); intros. clear H0. destruct H2.
+    specialize(Forall_cons_iff (fun Q : process =>
+       forall (X m l k : fin) (tm : option ltt) (Gs : ctxS) (Gtl Gtr : seq (option ltt))
+         (T : ltt),
+       typ_proc Gs (Gtl ++ Gtr) (incr_free l k X m Q) T ->
+       length Gtl = l -> typ_proc Gs (Gtl ++ tm :: Gtr) (incr_free l k X.+1 m Q) T)  a llp); intros. destruct H3. clear H4.
+    specialize(H3 H); intros. clear H. destruct H3.
+    specialize(IHllp x2 x4 X m k l Gs Gtl Gtr tm H3 H2 H1); intros. clear H2 H3.
+    apply Forall2_cons; try easy.
+    apply H. easy. easy.
+Qed. 
+
+Lemma onth_more {A} : forall l Gtl Gtr n X x (tm : option A),
+      (l <= n) = true ->
+      length Gtl = l ->
+      onth (n + X)%coq_nat (Gtl ++ Gtr) = Some x ->
+      Some x = onth (n + X.+1)%coq_nat (Gtl ++ tm :: Gtr).
+Proof.
+  intro l. induction l; intros; try easy.
+  - specialize(length_zero_iff_nil Gtl); intros. destruct H2. specialize(H2 H0); intros. clear H3. subst.
+    simpl.
+    specialize(Nat.add_succ_r n X); intros. replace ((n + X.+1)%coq_nat) with ((n + X)%coq_nat.+1). simpl.
+    simpl in H1. easy.
+  - destruct n. easy.
+    specialize(positive_list_length_dst Gtl l H0); intros.
+    destruct H2. destruct H2. replace Gtl with (x0 :: x1) in *. clear H2.
+    simpl in *.
+    apply IHl; try easy.
+    apply Nat.succ_inj. easy.
+Qed.
+
+Lemma onth_less {A} : forall l Gtl Gtr n x (tm : option A),
+      (l <= n) = false ->
+      length Gtl = l ->
+      onth n (Gtl ++ Gtr) = Some x ->
+      Some x = onth n (Gtl ++ tm :: Gtr).
+Proof.
+  intro l. induction l; intros; try easy.
+  specialize(positive_list_length_dst Gtl l H0); intros.
+  destruct H2. destruct H2. replace Gtl with (x0 :: x1) in *. 
+  destruct n; try easy.
+  simpl in *.
+  apply IHl; try easy.
+  apply Nat.succ_inj. easy.
+Qed.
+
+Lemma slideTp : forall Q X m l k tm Gs Gtl Gtr T,
+typ_proc Gs (Gtl ++ Gtr) (incr_free l k X m Q) T -> length Gtl = l -> typ_proc Gs (Gtl ++ [tm] ++ Gtr) (incr_free l k X.+1 m Q) T.
+Proof.
+  intro Q.
+  induction Q using process_ind_ref; intros; try easy.
+  - simpl in *. 
+    specialize(_a23_e (p_var (if l <= n then (n + X)%coq_nat else n)) (if l <= n then (n + X)%coq_nat else n) T Gs (Gtl ++ Gtr) H (erefl (p_var (if l <= n then (n + X)%coq_nat else n)))); intros.
+    destruct H1. destruct H1.
+    case_eq (l <= n); intros.
+    - replace (l <= n) with true in H, H1.
+      apply tc_sub with (t := x); try easy. 
+      apply tc_var; try easy.
+      apply onth_more with (l := l); try easy.
+    - replace (l <= n) with false in H, H1.
+      apply tc_sub with (t := x); try easy.
+      apply tc_var; try easy.
+      apply onth_less with (l := l); try easy.
+  - simpl in *. 
+    specialize(_a23_f p_inact T Gs (Gtl++Gtr) H (erefl p_inact)); intros. subst. 
+    apply tc_inact.
+  - simpl in *.
+    specialize(_a23_bf pt lb (incr_freeE k m ex) (incr_free l k X m Q) (p_send pt lb (incr_freeE k m ex) (incr_free l k X m Q)) Gs (Gtl ++ Gtr) T H (erefl (p_send pt lb (incr_freeE k m ex) (incr_free l k X m Q)))); intros.
+    destruct H1. destruct H1. destruct H1. destruct H2.
+    apply tc_sub with (t := (ltt_send pt [(lb, (x, x0))])); try easy.
+    apply tc_send; try easy.
+    apply IHQ. easy. easy.
+  - simpl in *.
+    specialize(_a23_a pt llb (list_map (incr_free l k.+1 X m) llp) (p_recv pt llb (list_map (incr_free l k.+1 X m) llp)) Gs (Gtl ++ Gtr) T H0 (erefl (p_recv pt llb (list_map (incr_free l k.+1 X m) llp)))); intros.
+    destruct H2. destruct H2. destruct H2. destruct H3. destruct H4. destruct H5. destruct H6.
+    apply tc_sub with (t := (ltt_recv pt (zip llb (zip x0 x)))); try easy.
+    
+    specialize(eq_trans (esym H2) H3); intros; try easy.
+    specialize(map_length (incr_free l k.+1 X m) llp); intros.
+    specialize(map_length (incr_free l k.+1 X.+1 m) llp); intros.
+    specialize(eq_trans H4 H9); intros.
+    specialize(eq_trans H11 (esym H10)); intros.
+    specialize(eq_trans (esym H3) H11); intros.
+    specialize(eq_trans H13 (esym H10)); intros.
+    apply tc_recv; try easy. clear H2 H3 H4 H6 H8 H9 H10 H11 H12 H13 H14.
+    apply slideT_helper; try easy.
+  - simpl in *.
+    specialize(_a23_c (p_ite (incr_freeE k m e) (incr_free l k X m Q1) (incr_free l k X m Q2)) (incr_freeE k m e) (incr_free l k X m Q1) (incr_free l k X m Q2) T Gs (Gtl ++ Gtr) H (erefl (p_ite (incr_freeE k m e) (incr_free l k X m Q1) (incr_free l k X m Q2)))); intros.
+    destruct H1. destruct H1. destruct H1. destruct H2. destruct H3. destruct H4.
+    apply tc_ite; try easy.
+    apply tc_sub with (t := x); try easy.
+    apply IHQ1; try easy.
+    apply tc_sub with (t := x0); try easy.
+    apply IHQ2; try easy. 
+  - simpl in *. 
+    specialize(_a23_d (p_rec (incr_free l.+1 k X m Q)) (incr_free l.+1 k X m Q) T Gs (Gtl++Gtr) H (erefl (p_rec (incr_free l.+1 k X m Q)))); intros.
+    destruct H1. destruct H1. destruct H1. destruct H2.
+    specialize(IHQ X m l.+1 k tm Gs (Some x :: Gtl) Gtr x0); intros.
+    specialize(cat_cons (Some x) Gtl Gtr); intros.
+    replace ((Some x :: Gtl) ++ Gtr) with (Some x :: Gtl ++ Gtr) in IHQ. clear H4.
+    specialize(IHQ H1); intros. simpl in IHQ.
+    specialize(eq_S (length Gtl) l H0); intros.
+    specialize(IHQ H4). clear H0 H4.
+    apply tc_sub with (t := x0); try easy.
+    apply tc_mu with (t := x); try easy.
+Qed.
+
+Lemma slideT : forall Q X m tm Gs Gt T,
+typ_proc Gs Gt (incr_free 0 0 X m Q) T -> typ_proc Gs (tm :: Gt) (incr_free 0 0 X.+1 m Q) T.
 Proof.
   intros.
-  specialize(trivial_type_inact em Gs (extendT Gt X T) T' H); intros. subst.
-  specialize(tc_inact em Gs Gt); intros.
-  specialize(_typ_consistency_ em Gs (extendT Gt X T) p_inact ltt_end H); intros.
-  destruct H1. simpl in H2. destruct H2.
-  specialize(H0 H1 H3); intros.
-  easy.
+  specialize(slideTp Q X m 0 0 tm Gs [] Gt T H); intros. simpl in H0.
+  apply H0; try easy.
 Qed.
 
-Lemma remove_unusedT_var : forall em Gs Gt X Y T T',
-  Y <> X -> typ_proc em Gs (extendT Gt X T) (p_var Y) T' -> typ_proc em Gs Gt (p_var Y) T'.
+Lemma slideSp_e : forall k m ex x Gsl Gsr tm,
+  typ_expr (Gsl ++ Gsr) (incr_freeE k m ex) x ->
+  length Gsl = k ->
+  typ_expr (Gsl ++ tm :: Gsr) (incr_freeE k m.+1 ex) x.
+Proof. 
+  intros k m ex. revert k m. induction ex; intros; try easy.
+  - simpl in *. 
+    specialize(inv_expr_var (e_var (if k <= n then (n + m)%coq_nat else n)) (if k <= n then (n + m)%coq_nat else n) (Gsl ++ Gsr) x H (erefl (e_var (if k <= n then (n + m)%coq_nat else n)))); intros.
+    destruct H1. destruct H1.
+    apply sc_sub with (s := x0); try easy.
+    apply sc_var.
+    case_eq (k <= n); intros.
+    - replace (k <= n) with true in H1. subst.
+      apply onth_more with (l := length Gsl); try easy.
+    - replace (k <= n) with false in H1. subst.
+      apply onth_less with (l := length Gsl); try easy.
+  - simpl in *. 
+    specialize(inv_expr_vali (Gsl ++ Gsr) (e_val v) x v H (erefl (e_val v))); intros.
+    destruct H1.
+    - subst. destruct H1. destruct H0. subst. apply sc_vali.
+    - subst. destruct H1. destruct H0. destruct H0. subst.
+      inversion H0. subst. apply sc_sub with (s := snat); try easy. apply sc_valn.
+      subst. apply sc_valn.
+    - subst. destruct H0. destruct H0. subst. apply sc_valb.
+  - simpl in *.
+    specialize(inv_expr_succ (Gsl ++ Gsr) (e_succ (incr_freeE k m ex)) x (incr_freeE k m ex) H (erefl (e_succ (incr_freeE k m ex)))); intros.
+    destruct H1. destruct H2.
+    - subst. apply sc_succ; try easy. apply IHex; try easy.
+    - subst. apply sc_sub with (s := snat); try easy. apply sc_succ; try easy. apply IHex; try easy.
+      apply sni.
+  - simpl in *.
+    specialize(inv_expr_neg (Gsl ++ Gsr) (e_neg (incr_freeE k m ex)) x (incr_freeE k m ex) H (erefl (e_neg (incr_freeE k m ex)))); intros.
+    destruct H1. subst. apply sc_neg. apply IHex; try easy.
+  - simpl in *.
+    specialize(inv_expr_not (Gsl ++ Gsr) (e_not (incr_freeE k m ex)) x (incr_freeE k m ex) H (erefl (e_not (incr_freeE k m ex)))); intros. 
+    destruct H1. subst. apply sc_not. apply IHex; try easy.
+  - simpl in *.
+    specialize(inv_expr_gt (Gsl ++ Gsr) (e_gt (incr_freeE k m ex1) (incr_freeE k m ex2)) x (incr_freeE k m ex1) (incr_freeE k m ex2) H (erefl (e_gt (incr_freeE k m ex1) (incr_freeE k m ex2)))); intros.
+    destruct H1. destruct H2.
+    subst. apply sc_gt. apply IHex1; try easy. apply IHex2; try easy.
+  - simpl in *.
+    specialize(inv_expr_plus (Gsl ++ Gsr) (e_plus (incr_freeE k m ex1) (incr_freeE k m ex2)) x (incr_freeE k m ex1) (incr_freeE k m ex2) H (erefl (e_plus (incr_freeE k m ex1) (incr_freeE k m ex2)))); intros.
+    destruct H1. destruct H2.
+    subst. apply sc_plus. apply IHex1; try easy. apply IHex2; try easy.
+Qed.
+
+Lemma slideS_helper : forall llp l k X m x0 x Gsl Gsr Gt tm,
+    length Gsl = k ->
+    Forall
+          (fun Q : process =>
+           forall (X m l k : fin) (tm : option sort) (Gsl Gsr : seq (option sort)) (Gt : ctxT) (T : ltt),
+           typ_proc (Gsl ++ Gsr) Gt (incr_free l k X m Q) T ->
+           length Gsl = k -> typ_proc (Gsl ++ tm :: Gsr) Gt (incr_free l k X m.+1 Q) T) llp ->
+    Forall2 (fun (u : process) (v : sort * ltt) => typ_proc (Some v.1 :: Gsl ++ Gsr) Gt u v.2)
+           (list_map (incr_free l k.+1 X m) llp) (zip x0 x) ->
+    Forall2 (fun (u : process) (v : sort * ltt) => typ_proc (Some v.1 :: Gsl ++ tm :: Gsr) Gt u v.2)
+      (list_map (incr_free l k.+1 X m.+1) llp) (zip x0 x).
+Proof.
+  intro llp. induction llp; intros; try easy.
+  - specialize(Forall2_length H1); intros. simpl in *.
+    specialize(length_zero_iff_nil (zip x0 x)); intros. destruct H3.
+    specialize(H3 (esym H2)). clear H2 H4. replace (zip x0 x) with (@nil (sort * ltt)). easy.
+  - specialize(Forall2_length H1); intros. simpl in *.
+    specialize(positive_list_length_dst_zip x0 x (length (list_map (incr_free l k.+1 X m) llp)) (esym H2)); intros.
+    destruct H3. destruct H3. destruct H3. destruct H3. 
+    replace (zip x0 x) with ((x1,x3) :: zip x2 x4) in *. clear H2 H3.
+    specialize(Forall2_cons_iff (fun (u : process) (v : sort * ltt) => typ_proc (Some v.1 :: Gsl ++ Gsr) Gt u v.2) (incr_free l k.+1 X m a) (x1,x3) (list_map (incr_free l k.+1 X m) llp) (zip x2 x4)); intros.
+    destruct H2. clear H3. specialize(H2 H1); intros. clear H1. destruct H2.
+    specialize(Forall_cons_iff (fun Q : process =>
+        forall (X m l k : fin) (tm : option sort) (Gsl Gsr : seq (option sort)) (Gt : ctxT) (T : ltt),
+        typ_proc (Gsl ++ Gsr) Gt (incr_free l k X m Q) T ->
+        length Gsl = k -> typ_proc (Gsl ++ tm :: Gsr) Gt (incr_free l k X m.+1 Q) T) a llp); intros.
+    destruct H3. specialize(H3 H0); intros. clear H4 H0. destruct H3.
+    specialize(IHllp l k X m x2 x4 Gsl Gsr Gt tm H H3 H2); intros. 
+    specialize(H0 X m l k.+1 tm (Some (x1, x3).1 :: Gsl) Gsr Gt (x1, x3).2); intros.
+    apply Forall2_cons; try easy.
+    apply H0; try easy. simpl.
+    apply eq_S. easy.
+Qed.
+
+Lemma slideSp : forall Q X m l k tm Gsl Gsr Gt T,
+typ_proc (Gsl ++ Gsr) Gt (incr_free l k X m Q) T -> length Gsl = k -> typ_proc (Gsl ++ [tm] ++ Gsr) Gt (incr_free l k X m.+1 Q) T.
+Proof.
+  intro Q.
+  induction Q using process_ind_ref; intros; try easy.
+  - simpl in *. 
+    specialize(_a23_e (p_var (if l <= n then (n + X)%coq_nat else n)) (if l <= n then (n + X)%coq_nat else n) T (Gsl ++ Gsr) Gt H (erefl (p_var (if l <= n then (n + X)%coq_nat else n)))); intros.
+    destruct H1. destruct H1.
+    apply tc_sub with (t := x); try easy. 
+    apply tc_var; try easy.
+  - simpl in *. 
+    specialize(_a23_f p_inact T (Gsl ++ Gsr) Gt H (erefl p_inact)); intros. subst.
+    apply tc_inact.
+  - simpl in *.
+    specialize(_a23_bf pt lb (incr_freeE k m ex) (incr_free l k X m Q) (p_send pt lb (incr_freeE k m ex) (incr_free l k X m Q)) (Gsl ++ Gsr) Gt T H (erefl (p_send pt lb (incr_freeE k m ex) (incr_free l k X m Q) ))); intros.
+    destruct H1. destruct H1. destruct H1. destruct H2.
+    apply tc_sub with (t := (ltt_send pt [(lb, (x, x0))])); try easy.
+    apply tc_send; try easy.
+    apply slideSp_e; try easy.
+    apply IHQ; try easy. 
+  - simpl in *.
+    specialize(_a23_a pt llb (list_map (incr_free l k.+1 X m) llp) (p_recv pt llb (list_map (incr_free l k.+1 X m) llp)) (Gsl ++ Gsr) Gt T H0 (erefl (p_recv pt llb (list_map (incr_free l k.+1 X m) llp)))); intros.
+    destruct H2. destruct H2. destruct H2. destruct H3. destruct H4. destruct H5. destruct H6.
+    apply tc_sub with (t := (ltt_recv pt (zip llb (zip x0 x)))); try easy.
+    specialize(eq_trans (esym H2) H3); intros.
+    specialize(map_length (incr_free l k.+1 X m) llp); intros.
+    specialize(map_length (incr_free l k.+1 X m.+1) llp); intros.
+    specialize(eq_trans H4 H9); intros.
+    specialize(eq_trans H11 (esym H10)); intros.
+    specialize(eq_trans (esym H3) H12); intros.
+    apply tc_recv; try easy. clear H2 H3 H4 H6 H8 H9 H10 H11 H12 H13.
+    apply slideS_helper; try easy.
+  - simpl in *.
+    specialize(_a23_c (p_ite (incr_freeE k m e) (incr_free l k X m Q1) (incr_free l k X m Q2)) (incr_freeE k m e) (incr_free l k X m Q1) (incr_free l k X m Q2) T (Gsl ++ Gsr) Gt H (erefl (p_ite (incr_freeE k m e) (incr_free l k X m Q1) (incr_free l k X m Q2)))); intros.
+    destruct H1. destruct H1. destruct H1. destruct H2. destruct H3. destruct H4.
+    apply tc_ite; try easy.
+    apply slideSp_e; try easy.
+    apply tc_sub with (t := x); try easy. apply IHQ1; try easy.
+    apply tc_sub with (t := x0); try easy. apply IHQ2; try easy.
+  - simpl in *.
+    specialize(_a23_d (p_rec (incr_free l.+1 k X m Q)) (incr_free l.+1 k X m Q) T (Gsl ++ Gsr) Gt H (erefl (p_rec (incr_free l.+1 k X m Q)))); intros.
+    destruct H1. destruct H1. destruct H1. destruct H2.
+    apply tc_sub with (t := x0); try easy.
+    apply tc_mu with (t := x); try easy.
+    apply IHQ; try easy.
+Qed.
+
+Lemma slideS : forall Q X m tm Gs Gt T,
+typ_proc Gs Gt (incr_free 0 0 X m Q) T -> typ_proc (tm :: Gs) Gt (incr_free 0 0 X m.+1 Q) T.
 Proof.
   intros.
-  specialize(_a23_e (p_var Y) em Y T' Gs (extendT Gt X T) H0 (eq_refl (p_var Y))); intros.
-  destruct H1. destruct H1. destruct H1.
-  unfold eq_ctxT in H1.
-  specialize(H1 Y); intros. simpl in H1.
-  destruct H1. destruct H1. destruct H3. destruct H3.
-  specialize(Nat.eqb_refl Y); intros.
-  replace (Y =? Y)%nat with true in H5.
-  specialize(Nat.eqb_neq Y X); intros. destruct H8. specialize(H9 H); intros.
-  replace (Y =? X)%nat with false in H5.
-  
-  specialize(tc_var em Gs Gt Y x); intros.
-  specialize(_typ_consistency_ em Gs (extendT Gt X T) (p_var Y) T' H0); intros.
-  destruct H11. simpl in H12. destruct H12.
-  specialize(H10 H11 H13 H5); intros.
-  specialize(tc_sub em Gs Gt (p_var Y) x T' H10 H2); intros.
-  easy.
+  specialize(slideSp Q X m 0 0 tm [] Gs Gt T H); intros. simpl in H0.
+  apply H0; try easy.
 Qed.
 
-(* Lemma alphaP_typ_eq {P Q : process} {em : fin} {Gs : ctxS} {Gt : ctxT} {T : ltt} :
-      alphaP P Q -> typ_proc em Gs Gt P T -> typ_proc em Gs Gt Q T.
-      intros.
-      induction H; intros; try easy.
-Admitted.
- *)
-(* 
-Theorem typ_proc_ind:
-  forall {em:fin} (P:list X -> Prop),
-    P nil ->
-    (forall x l, P l -> P (rcons l x)) ->
-    forall l, P l.
-Proof. Admitted.
-
- *)
-
-Lemma inv_subst_var : forall x P Q1 Q2 n, wtyped P -> wtyped Q1 -> wtyped Q2 -> substitutionP x P Q1 Q2 -> Q1 = (p_var n)
-                 -> (x = n /\ alphaP P Q2) \/ (x <> n /\ Q2 = p_var n).
+Lemma _a21_recv_helper : forall llp X m n Q T Gs Gt x x0 ys,
+  wtyped Q ->
+  onth X Gt = None ->
+  typ_proc Gs Gt (incr_free 0 0 m n Q) T ->
+  Forall
+      (fun P : process =>
+       forall (Q : process) (T T' : ltt) (Gs : ctxS) (Gt : ctxT) 
+         (X : fin) (Q' : process) (m n : fin),
+       wtyped Q ->
+       typ_proc Gs (extendT X T Gt) P T' ->
+       onth X Gt = None ->
+       substitutionP X m n Q P Q' ->
+       typ_proc Gs Gt (incr_free 0 0 m n Q) T -> typ_proc Gs Gt Q' T') llp ->
+  Forall2
+        (fun (u : process) (v : sort * ltt) =>
+         typ_proc (Some v.1 :: Gs) (extendT X T Gt) u v.2) llp 
+        (zip x0 x) ->
+  Forall2 (substitutionP X m n.+1 Q) llp ys ->
+  Forall2 (fun (u : process) (v : sort * ltt) => typ_proc (Some v.1 :: Gs) Gt u v.2) ys
+  (zip x0 x).
 Proof.
-  intros x P Q1 Q2 n WP WQ1 WQ2 H.
-  induction H using substitutionP_ind_ref; intros; try easy.
-  inversion H. subst. left. split. easy. 
-  specialize(alphaP_refl Pr); intros. easy.
-  right. inversion H0. subst. split. easy. easy.
-  specialize(IHsubstitutionP WP); intros.
-  specialize(wtyped_alphaP P2 P1 (alphaP_sym P1 P2 H) WQ1); intros.
-  subst. specialize(inv_alphaP_var P1 n H); intros. subst.
-  specialize(wtyped_alphaP Q2 Q1 (alphaP_sym Q1 Q2 H0) WQ2); intros.
-  specialize(IHsubstitutionP H2 H1 (ssrfun.erefl (p_var n))); intros.
-  destruct IHsubstitutionP. 
-  - left. split. destruct H3. easy. admit.
-  - right. split. destruct H3. easy. admit.
+  intro llp. induction llp; intros; try easy.
+  specialize(Forall2_length H3); intros. simpl in H5.
+  specialize(Forall2_length H4); intros. simpl in H6.
+  specialize(length_zero_iff_nil (zip x0 x)); intros. destruct H7. specialize(H7 (esym H5)); intros.
+  specialize(length_zero_iff_nil ys); intros. destruct H9. specialize(H9 (esym H6)); intros.
+  subst. replace (zip x0 x) with (@nil (sort * ltt)). easy.
+  
+  specialize(Forall2_length H3); intros. simpl in H5.
+  specialize(positive_list_length_dst_zip x0 x (length llp) (esym H5)); intros.
+  destruct H6. destruct H6. destruct H6. destruct H6.
+  replace (zip x0 x) with ((x1, x3) :: zip x2 x4) in *. simpl in *.
+  specialize(Forall2_length H4); intros. simpl in H7.
+  specialize(positive_list_length_dst ys (length llp) (esym H7)); intros.
+  destruct H8. destruct H8. subst. clear H5 H6 H7.
+  specialize(Forall2_cons_iff (fun (u : process) (v : sort * ltt) =>
+       typ_proc (Some v.1 :: Gs) (extendT X T Gt) u v.2) a (x1,x3) llp (zip x2 x4)); intros.
+  destruct H5. specialize(H5 H3); intros. clear H6 H3. destruct H5.
+  specialize(Forall2_cons_iff (substitutionP X m n.+1 Q) a x5 llp x6); intros.
+  destruct H6. specialize(H6 H4); intros. clear H7 H4. destruct H6.
+  specialize(Forall_cons_iff (fun P : process =>
+        forall (Q : process) (T T' : ltt) (Gs : ctxS) (Gt : ctxT) 
+          (X : fin) (Q' : process) (m n : fin),
+        wtyped Q ->
+        typ_proc Gs (extendT X T Gt) P T' ->
+        onth X Gt = None ->
+        substitutionP X m n Q P Q' ->
+        typ_proc Gs Gt (incr_free 0 0 m n Q) T -> typ_proc Gs Gt Q' T') a llp); intros.
+  destruct H7. specialize(H7 H2); intros. clear H8 H2. destruct H7.
+  specialize(H2 Q T (x1, x3).2 (Some (x1, x3).1 :: Gs) Gt X x5 m n.+1 H H3 H0 H4); intros.
+  specialize(IHllp X m n Q T Gs Gt x4 x2 x6 H H0 H1 H7 H5 H6); intros.
+  apply Forall2_cons; try easy.
+  apply H2.
+  apply slideS; try easy.
+Qed. 
 
-Admitted.
- 
-Lemma inv_subst_inact : forall x P Q1 Q2, substitutionP x P Q1 Q2 -> (Q1 = p_inact) -> Q2 = p_inact.
-Proof.
-  intros x P Q1 Q2 Hs.
-  induction Hs using substitutionP_ind_ref; intros; try easy.
-  induction H using alphaP_ind_ref; intros; try easy. 
-  specialize(IHHs H1); intros; try easy.
-  subst. 
-  specialize(inv_alphaP_inact Q2); intros. 
-  specialize(alphaP_sym p_inact Q2 H0); intros.
-  specialize(H H2); intros; try easy.
-Qed.
+Lemma _a21: forall P Q T T' Gs Gt X Q' m n, wtyped Q 
+  -> typ_proc Gs (extendT X T Gt) P T' -> onth X Gt = None 
+  -> substitutionP X m n Q P Q' -> typ_proc Gs Gt (incr_free 0 0 m n Q) T
+  -> typ_proc Gs Gt Q' T'.
+Proof. 
 
-Lemma inv_subst_rec : forall P X Qb Qa, wtyped Qa -> wtyped Qb -> (exists n Q, P = (p_rec n Q)) -> substitutionP X Qb P Qa -> exists m Q', (Qa = p_rec m Q').
-Proof.
-  intros. revert H.  
-  induction H2 using substitutionP_ind_ref; intros; try easy.
-  destruct H1. destruct H1. easy.
-  destruct H1. destruct H1. easy.
-  destruct H1. destruct H1. easy.
-  destruct H1. destruct H1. easy.
+  intros P. induction P using process_ind_ref.
   
-  destruct H1. destruct H1. 
-  exists Y. exists Q1. easy.
+  (* var *)
   
-  destruct H1. destruct H1. subst. 
-  specialize(inv_alphaP_rec P1 x x0 H); intros. destruct H1. destruct H1. destruct H1. destruct H1. 
-  destruct H4. destruct H5. 
-  destruct IHsubstitutionP. easy. exists x1. exists x3. easy. 
-  specialize(wtyped_alphaP Q2 Q1 (alphaP_sym Q1 Q2 H2) H3); intros. easy.
+  intros.
+  inversion H2. subst.
+  specialize(_a23_e (p_var n) n T' Gs (extendT n T Gt) H0 (erefl (p_var n))); intros.
+  destruct H4. destruct H4.
+  specialize(extend_extract n T Gt); intros.
+  specialize(eq_trans (esym H4) H6); intros. inversion H7. subst.
+  apply tc_sub with (t := T); intros; try easy.
   
-  destruct H7. subst.  
-  specialize(inv_alphaP_rec Q2 x4 x5 (alphaP_sym (p_rec x4 x5) Q2 H2)); intros.
-  destruct H1. destruct H1. destruct H1. destruct H1.
-  exists x6. exists x8. easy.
+  subst.
+  specialize(_a23_e (p_var n) n T' Gs (extendT X T Gt) H0 (erefl (p_var n))); intros.
+  destruct H4. destruct H4.
+  apply tc_sub with (t := x); try easy.
+  apply tc_var.
+  apply ssrfun.esym. apply remove_var with (X := X) (T:= T); try easy.
+  
+  (* inact *)
+  intros.
+  inversion H2. subst.
+  specialize(_a23_f p_inact T' Gs (extendT X T Gt) H0 (erefl p_inact)); intros. subst.
+  apply tc_inact.
+  
+  (* send *)
+  intros. 
+  inversion H2. subst.
+  specialize(_a23_bf pt lb ex P (p_send pt lb ex P) Gs (extendT X T Gt) T' H0 (erefl (p_send pt lb ex P))); intros. 
+  destruct H4. destruct H4. destruct H4. destruct H5. 
+  specialize(IHP Q T x0 Gs Gt X Q'0 m n H H5 H1 H13 H3); intros.
+  apply tc_sub with (t := (ltt_send pt [(lb, (x, x0))])); try easy.
+  apply tc_send; try easy.
+  
+  (* recv *)
+  intros.
+  inversion H3. subst.
+  specialize(_a23_a pt llb llp (p_recv pt llb llp) Gs (extendT X T Gt) T' H1 (erefl (p_recv pt llb llp))); intros.
+  destruct H5. destruct H5. destruct H5. destruct H6. destruct H7. destruct H9. destruct H10.
+  apply tc_sub with (t := (ltt_recv pt (zip llb (zip x0 x)))); try easy.
+  specialize(eq_trans (esym H5) H6); intros.
+  specialize(eq_trans (esym H12) H13); intros.
+  specialize(eq_trans H5 H13); intros.
+  apply tc_recv; try easy.
+  apply _a21_recv_helper with (llp := llp) (m := m) (n := n) (Q := Q) (X := X) (T := T); try easy.
+  
+  (* ite *)
+  intros. 
+  inversion H2. subst.
+  specialize(_a23_c (p_ite e P1 P2) e P1 P2 T' Gs (extendT X T Gt) H0 (erefl (p_ite e P1 P2))); intros.
+  destruct H4. destruct H4. destruct H4. destruct H5. destruct H6. destruct H7. 
+  specialize(IHP1 Q T x Gs Gt X Q1 m n H H4 H1 H12 H3); intros.
+  specialize(IHP2 Q T x0 Gs Gt X Q2 m n H H5 H1 H13 H3); intros.
+  apply tc_ite; intros; try easy.
+  apply tc_sub with (t := x); intros; try easy.
+  apply tc_sub with (t := x0); intros; try easy. 
+    
+  (* rec *)
+  intros.
+  inversion H2. subst.
+  specialize(_a23_d (p_rec P) P T' Gs (extendT X T Gt) H0 (erefl (p_rec P))); intros.
+  destruct H4. destruct H4. destruct H4. destruct H5.
+  specialize(IHP Q T x0 Gs (Some x :: Gt) X.+1 Q'0 m.+1 n H H4 H1 H9); intros.
+  apply tc_sub with (t := x0); try easy.
+  apply tc_mu with (t := x); try easy.
+  apply IHP.
+  apply slideT; try easy. 
 Qed.
 
 Lemma Forall2_to_Forall {A B : Type} [P : A -> Prop] [P1 : list A] [P2 : list B] :
@@ -160,7 +507,7 @@ Proof.
   apply Forall_cons; try easy.
 Qed.
 
-Lemma typable_implies_wtyped [em : fin] [Gs : ctxS] [Gt : ctxT] [P : process] [T : ltt] : typ_proc em Gs Gt P T -> wtyped P.
+Lemma typable_implies_wtyped [Gs : ctxS] [Gt : ctxT] [P : process] [T : ltt] : typ_proc Gs Gt P T -> wtyped P.
 Proof.
   intros. induction H using typ_proc_ind_ref.
   apply wp_inact.
@@ -168,99 +515,61 @@ Proof.
   apply wp_rec. easy.
   apply wp_ite; try easy. easy.
   apply wp_recv; try easy. 
-  - specialize(eq_trans H H0); intros; try easy.
+  - specialize(eq_trans H H0); intros; try easy. 
     apply (Forall2_to_Forall H3).
-  apply wp_send; try easy.
-Qed.
-
-Lemma typable_after_subst_list [xs ys : list process] [Pr : process] : wtyped Pr -> Forall2 (fun Q1 Q2 : process => wtyped Pr -> wtyped Q1 -> wtyped Q2) xs ys -> Forall wtyped xs -> Forall wtyped ys.
-Proof.
-  revert ys.
-  induction xs.
-  - intros. specialize(Forall2_length H0); intros. 
-    simpl in H2.
-    specialize(length_zero_iff_nil ys); intros. destruct H3.
-    specialize(H3 (eq_sym H2)). subst. easy.
-  - intros. 
-    specialize(Forall2_length H0); intros. simpl in H2.
-    specialize(positive_list_length_dst ys (length xs) (eq_sym H2)); intros.
-    destruct H3. destruct H3. subst.
-    specialize(Forall2_cons_iff (fun Q1 Q2 : process => wtyped Pr -> wtyped Q1 -> wtyped Q2) a x xs x0); intros.
-    destruct H3. specialize(H3 H0). clear H4. destruct H3.
-    specialize(Forall_cons_iff wtyped a xs); intros. destruct H5.
-    specialize(H5 H1); intros. destruct H5. clear H6. 
-    specialize(H3 H H5); intros.
-    specialize(IHxs x0 H H4 H7); intros.
-    apply Forall_cons. easy. easy.
-Qed.
-
-Lemma typable_after_subst [X : fin] [P Q1 Q2 : process] : substitutionP X P Q1 Q2 -> wtyped P -> wtyped Q1 -> wtyped Q2.
-Proof.
-  intro H. induction H using substitutionP_ind_ref; intros; try easy.
-  - inversion H0. subst.
-    specialize(IHsubstitutionP H H2); intros.
     apply wp_send. easy.
-  - inversion H4. subst.
-    apply wp_recv; try easy.
-    specialize(typable_after_subst_list H3 H2 H10); intros. easy.
-  - inversion H0. subst.
-    apply wp_ite. 
-    specialize(IHsubstitutionP H H3); intros; try easy.
-    specialize(IHsubstitutionP0 H H5); intros; try easy.
-  - inversion H2. subst.
-    apply wp_rec. 
-    specialize(IHsubstitutionP H1 H4); intros; try easy.
-  - specialize(wtyped_alphaP P2 P1 (alphaP_sym P1 P2 H) H2); intros.
-    specialize(IHsubstitutionP H1 H3); intros.
-    specialize(wtyped_alphaP Q1 Q2 H0 IHsubstitutionP); intros. easy.
 Qed.
 
-Lemma typable_alpha [em : fin] [Gs : ctxS] [Gt : ctxT] [P1 P2 : process] [T : ltt] :
-      alphaP P1 P2 -> typ_proc em Gs Gt P1 T -> typ_proc em Gs Gt P2 T.
+Lemma trivial_incrE : forall n ex, (incr_freeE n 0 ex) = ex.
+Proof.
+  intros n ex. induction ex; intros; try easy.
+  - simpl. destruct (n <= n0); try easy.
+    specialize(Nat.add_0_r n0); intros. replace (n0 + 0)%coq_nat with n0. easy.
+  - simpl. replace (incr_freeE n 0 ex) with ex. easy.
+  - simpl. replace (incr_freeE n 0 ex) with ex. easy.
+  - simpl. replace (incr_freeE n 0 ex) with ex. easy.
+  - simpl. replace (incr_freeE n 0 ex1) with ex1. replace (incr_freeE n 0 ex2) with ex2. easy.
+  - simpl. replace (incr_freeE n 0 ex1) with ex1. replace (incr_freeE n 0 ex2) with ex2. easy.
+Qed.
+
+Lemma trivial_incr : forall m n Q, (incr_free m n 0 0 Q) = Q.
+Proof.
+  intros. revert m n. induction Q using process_ind_ref; intros; simpl; try easy. 
+  - destruct (m <= n); try easy.
+    specialize(Nat.add_0_r n); intros. replace (n + 0)%coq_nat with n; easy.
+  - specialize(trivial_incrE n ex); intros.
+    specialize(IHQ m n); intros.
+    replace (incr_freeE n 0 ex) with ex. replace (incr_free m n 0 0 Q) with Q. easy.
+  - assert (list_map (incr_free m n.+1 0 0) llp = llp).
+    {
+      induction llp. easy.
+      specialize(Forall_cons_iff (fun Q : process => forall m n : fin, incr_free m n 0 0 Q = Q) a llp); intros.
+      destruct H0. specialize(H0 H); intros. clear H1 H. destruct H0.
+      specialize(IHllp H0); intros.
+      simpl.
+      specialize(H m n.+1); intros.
+      replace (incr_free m n.+1 0 0 a) with a.
+      replace (list_map (incr_free m n.+1 0 0) llp) with llp. easy.
+    }
+    replace (list_map (incr_free m n.+1 0 0) llp) with llp. easy.
+  - specialize(trivial_incrE n e); intros. 
+    specialize(IHQ1 m n); intros. specialize(IHQ2 m n); intros.
+    replace (incr_freeE n 0 e) with e.
+    replace (incr_free m n 0 0 Q1) with Q1. 
+    replace (incr_free m n 0 0 Q2) with Q2.
+    easy.
+  - specialize(IHQ m.+1 n); intros. 
+    replace (incr_free m.+1 n 0 0 Q) with Q. easy.
+Qed.
+
+Lemma _a21f : forall P Q T T' Gs Gt X Q',
+     typ_proc Gs (extendT X T Gt) P T' -> onth X Gt = None 
+  -> substitutionP X 0 0 Q P Q' -> typ_proc Gs Gt Q T
+  -> typ_proc Gs Gt Q' T'.
 Proof.
   intros.
-  induction H0 using typ_proc_ind_ref.
-Admitted.
-  
-
-Lemma _a21: forall P Q em T T' Gs Gt X Q', wtyped Q -> subtypeC T T'
-  -> typ_proc em Gs (extendT Gt X T) P T' -> typ_proc em Gs Gt Q T' 
-  -> substitutionP X Q P Q'
-  -> typ_proc em Gs Gt Q' T'.
-Proof. 
-
-  intros P. induction P using process_ind_ref.
-  
-  (* var *)
-  
-  intros.
-  specialize(inv_subst_var X Q (p_var n) Q' n); intros.
-  specialize(typable_implies_wtyped H1); intros.
-  specialize(typable_after_subst H3 H H5); intros.
-  specialize(H4 H H5 H6 H3); intros.
-  destruct H4. easy.
-  destruct H4. 
-  specialize(typable_alpha H7 H2); intros; try easy.
-  destruct H4. subst.
-  specialize(remove_unusedT_var em Gs Gt X n T T' (not_eq_sym H4) H1); intros. easy.  
-  
-  (* inact *)
-  intros.
-  specialize(inv_subst_inact X Q p_inact Q' H3 (eq_refl p_inact)); intros. subst.
-  specialize(remove_unusedT_inact em Gs Gt X T T' H1); intros. easy.
-  
-  (* send *)
-  intros.
-  
-  (* recv *)
-  
-  
-  (* ite *)
-  
-  
-  (* rec *)
-  
-  
-   
-Admitted.
-
+  apply _a21 with (P := P) (Q := Q) (T := T) (X := X) (m := 0) (n := 0); try easy.
+  apply typable_implies_wtyped with (Gs := Gs) (Gt := Gt) (T := T). easy.
+  specialize(trivial_incr 0 0 Q); intros. 
+  replace (incr_free 0 0 0 0 Q) with Q. easy.
+Qed.
