process/typecheck.v
@@ -5,54 +5,27 @@ From mathcomp Require Import ssreflect.seq.
 Import ListNotations.
 From Paco Require Import paco.
 
-Inductive ctxS : Type := 
-  | emptyS : ctxS
-  | consS : fin -> sort -> ctxS -> ctxS.
 
-Inductive ctxT : Type := 
-  | emptyT : ctxT 
-  | consT : fin -> ltt -> ctxT -> ctxT.
+Definition ctxS := list (option sort).
+Definition ctxT := list (option ltt).
 
-Definition extendS (m: ctxS) (s: fin) (t: expressions.sort) :=
-  consS s t m.
-
-Definition extendT (m: ctxT) (s: fin) (t: ltt) :=
-  consT s t m.
-
-Fixpoint lookupS (m: ctxS) (s: fin): option expressions.sort :=
-  match m with
-    | consS s' t' xs => if Nat.eqb s s' then Some t' else lookupS xs s
-    | emptyS          => None
+Fixpoint onth {A : Type} (n : fin) (lis : list (option A)) : option A :=
+  match lis with 
+    | x::xs =>
+      match n with
+        | S m => onth m xs
+        | 0   => x
+      end
+    | [] => None
   end.
-
-Fixpoint lookupT (m: ctxT) (s: fin): option ltt :=
-  match m with
-    | consT s' t' xs => if Nat.eqb s s' then Some t' else lookupT xs s
-    | emptyT          => None
-  end.
-
-Fixpoint consistent_ctxS (m : ctxS) : Prop := 
-  match m with 
-    | emptyS => True
-    | consS f _ l => (lookupS l f = None) /\ consistent_ctxS l
-  end.
-
-Fixpoint consistent_ctxT (m : ctxT) : Prop := 
-  match m with 
-    | emptyT => True
-    | consT f _ l => (lookupT l f = None) /\ consistent_ctxT l
-  end.
-  
-Definition eq_ctxS (m1 m2 : ctxS) := forall n, consistent_ctxS m1 /\ consistent_ctxS m2 /\ lookupS m1 n = lookupS m2 n.
-Definition eq_ctxT (m1 m2 : ctxT) := forall n, consistent_ctxT m1 /\ consistent_ctxT m2 /\ lookupT m1 n = lookupT m2 n.
 
 
 Inductive typ_expr: ctxS -> expr -> sort -> Prop :=
-  | sc_var : forall c s t, consistent_ctxS c -> Some t = lookupS c s -> typ_expr c (e_var s) t
-  | sc_vali: forall c i, consistent_ctxS c -> typ_expr c (e_val (vint i)) sint
-  | sc_valn: forall c i, consistent_ctxS c -> typ_expr c (e_val (vnat i)) snat
-  | sc_valb: forall c b, consistent_ctxS c -> typ_expr c (e_val (vbool b)) sbool
-  | sc_succ: forall c e, consistent_ctxS c -> typ_expr c e snat ->
+  | sc_var : forall c s t, Some t = onth s c -> typ_expr c (e_var s) t
+  | sc_vali: forall c i, typ_expr c (e_val (vint i)) sint
+  | sc_valn: forall c i, typ_expr c (e_val (vnat i)) snat
+  | sc_valb: forall c b, typ_expr c (e_val (vbool b)) sbool
+  | sc_succ: forall c e, typ_expr c e snat ->
                          typ_expr c (e_succ e) snat
   | sc_neg : forall c e, typ_expr c e sint ->
                          typ_expr c (e_neg e) sint
@@ -68,90 +41,61 @@ Inductive typ_expr: ctxS -> expr -> sort -> Prop :=
                              typ_expr c e2 sint ->
                              typ_expr c (e_plus e1 e2) sint.
 
-Fixpoint matchSel (l: label) (xs: list(label*(expressions.sort)*ltt)%type): option ((sort)*ltt)%type :=
-  match xs with
-    | nil           => None
-    | (lbl,s,t)::ys => if Nat.eqb l lbl then Some(s,t) else matchSel l ys
-  end.
 
-(* Require Import Coq.Init.Logic. *)
-
-(* Definition sub_ctx (m1 m2: ctx) :=
-  ((forall n s s', subsort s s'  -> (memS n s m1 <-> memS n s' m2)) \/ eq_ctx m1 m2) /\
-  ((forall n t t', subtypeC t t' -> (memT n t m1 <-> memT n t' m2)) \/ eq_ctx m1 m2). *)
-
-Definition IF_then_else (P Q R:Prop) := P /\ Q \/ ~ P /\ R.
-
-Fixpoint findCtxT (n: fin) (t: ltt) (m: ctxT): Prop :=
-  match m with
-    | consT u v m1 => (n = u /\ v = t) \/ findCtxT n t m1
-    | _            => False
-  end.
-
-Search (Forall2).
-
-(* Inductive Forall5 : forall [A B C D E : Type], (A -> B -> C -> D -> E -> Prop) -> seq A -> seq B -> seq C -> seq D -> seq E -> Prop :=
-  | Forall5_nil  : forall [A B C D E : Type] (R : A -> B -> C -> D -> E -> Prop), Forall5 R [] [] [] [] []
-  | Forall5_cons : forall [A B C D E : Type] [R : A -> B -> C -> D -> E -> Prop] (a : A) (b : B) (c : C) (d : D) (e : E) [l0 : seq A] [l1 : seq B] [l2 : seq C] [l3 : seq D] [l4 : seq E], R a b c d e -> Forall5 R l0 l1 l2 l3 l4 -> Forall5 R (a :: l0) (b :: l1) (c :: l2) (d :: l3) (e :: l4).
-  
-Inductive Forall3 : forall [A B C : Type], (A -> B -> C -> Prop) -> seq A -> seq B -> seq C -> Prop :=
-  | Forall3_nil  : forall [A B C : Type] (R : A -> B -> C -> Prop), Forall3 R [] [] []
-  | Forall3_cons : forall [A B C : Type] [R : A -> B -> C -> Prop] (a : A) (b : B) (c : C) [l0 : seq A] [l1 : seq B] [l2 : seq C], R a b c -> Forall3 R l0 l1 l2 -> Forall3 R (a :: l0) (b :: l1) (c :: l2). *)
-
-Inductive typ_proc: fin -> ctxS -> ctxT -> process -> ltt -> Prop :=
-  | tc_inact: forall em cs ct, consistent_ctxS cs -> consistent_ctxT ct -> typ_proc em cs ct (p_inact) (ltt_end)
-  | tc_var  : forall em cs ct s t, consistent_ctxS cs -> consistent_ctxT ct -> Some t = lookupT ct s ->
-                                   typ_proc em cs ct (p_var s) t
-  | tc_mu   : forall em cs ct x p t t', let ct' := extendT ct x t in
-                                     typ_proc em cs ct' p t ->
-                                     subtypeC t t' ->
-                                     typ_proc em cs ct (p_rec x p) t'
-  | tc_ite  : forall em cs ct e p1 p2 T, typ_expr cs e sbool ->
-                                         typ_proc em cs ct p1 T ->
-                                         typ_proc em cs ct p2 T ->
-                                         typ_proc em cs ct (p_ite e p1 p2) T
-  | tc_sub  : forall em cs ct p t t', typ_proc em cs ct p t ->
-                                              subtypeC t t' ->
-                                              typ_proc em cs ct p t'
-  | tc_recv : forall em cs ct p L ST P T,
+(*  depth *)
+Inductive typ_proc: ctxS -> ctxT -> process -> ltt -> Prop :=
+  | tc_inact: forall cs ct,     typ_proc cs ct (p_inact) (ltt_end)
+  | tc_var  : forall cs ct s t, Some t = onth s ct ->
+                                typ_proc cs ct (p_var s) t
+  | tc_mu   : forall cs ct p t t',    typ_proc cs (Some t :: ct) p t' ->
+                                      subtypeC t t' ->
+                                      typ_proc cs ct (p_rec p) t'
+  | tc_ite  : forall cs ct e p1 p2 T, typ_expr cs e sbool ->
+                                      typ_proc cs ct p1 T ->
+                                      typ_proc cs ct p2 T ->
+                                      typ_proc cs ct (p_ite e p1 p2) T
+  | tc_sub  : forall cs ct p t t',    typ_proc cs ct p t ->
+                                      subtypeC t t' ->
+                                      typ_proc cs ct p t'
+  | tc_recv : forall cs ct p L ST P T,
                      length L = length ST ->
                      length ST = length P ->
                      length P = length T ->
                      SSortedNList L ->
-                     Forall2 (fun u v => typ_proc (S em) (extendS cs em (fst v)) ct u (snd v)) P (zip ST T) ->
-                     typ_proc em cs ct (p_recv p L P) (ltt_recv p (zip (zip L ST) T))
-  | tc_send: forall em cs ct p l e P S T, typ_expr cs e S ->
-                                          typ_proc em cs ct P T ->
-                                          typ_proc em cs ct (p_send p l e P) (ltt_send p [(l,S,T)]).
+                     Forall2 (fun u v => typ_proc (Some (fst v) :: cs) ct u (snd v)) P (zip ST T) ->
+                     typ_proc cs ct (p_recv p L P) (ltt_recv p (zip L (zip ST T)))
+  | tc_send: forall cs ct p l e P S T, typ_expr cs e S ->
+                                       typ_proc cs ct P T ->
+                                       typ_proc cs ct (p_send p l e P) (ltt_send p [(l,(S,T))]).
 
 Print typ_proc_ind.
 
 Section typ_proc_ind_ref.
-  Variable P : fin -> ctxS -> ctxT -> process -> ltt -> Prop.
-  Hypothesis P_inact : forall em cs ct, consistent_ctxS cs -> consistent_ctxT ct -> P em cs ct p_inact ltt_end.
-  Hypothesis P_var   : forall em cs ct s t, consistent_ctxS cs -> consistent_ctxT ct -> Some t = lookupT ct s -> P em cs ct (p_var s) t.
-  Hypothesis P_mu    : forall em cs ct x p t t', let ct' := extendT ct x t in P em cs ct' p t -> subtypeC t t' -> P  em cs ct (p_rec x p) t'.
-  Hypothesis P_ite   : forall em cs ct e p1 p2 T, typ_expr cs e sbool -> P em cs ct p1 T -> P em cs ct p2 T -> P em cs ct (p_ite e p1 p2) T.
-  Hypothesis P_sub   : forall em cs ct p t t', P em cs ct p t -> subtypeC t t' -> P em cs ct p t'.
-  Hypothesis P_recv  : forall em cs ct p L ST Pr T, length L = length ST -> length ST = length Pr -> length Pr = length T ->
+  Variable P : ctxS -> ctxT -> process -> ltt -> Prop.
+  Hypothesis P_inact : forall cs ct, P cs ct p_inact ltt_end.
+  Hypothesis P_var   : forall cs ct s t, Some t = onth s ct -> P cs ct (p_var s) t.
+  Hypothesis P_mu    : forall cs ct p t t', P cs (Some t :: ct) p t' -> subtypeC t t' -> P cs ct (p_rec p) t'.
+  Hypothesis P_ite   : forall cs ct e p1 p2 T, typ_expr cs e sbool -> P cs ct p1 T -> P cs ct p2 T -> P cs ct (p_ite e p1 p2) T.
+  Hypothesis P_sub   : forall cs ct p t t', P cs ct p t -> subtypeC t t' -> P cs ct p t'.
+  Hypothesis P_recv  : forall cs ct p L ST Pr T, length L = length ST -> length ST = length Pr -> length Pr = length T ->
                      SSortedNList L ->
-                     List.Forall2 (fun u v => P (S em) (extendS cs em (fst v)) ct u (snd v)) Pr (zip ST T) ->
-                     P em cs ct (p_recv p L Pr) (ltt_recv p (zip (zip L ST) T)).
-  Hypothesis P_send  : forall em cs ct p l e Pr S T, typ_expr cs e S -> P em cs ct Pr T -> P em cs ct (p_send p l e Pr) (ltt_send p [(l,S,T)]).
+                     List.Forall2 (fun u v => P (Some (fst v) :: cs) ct u (snd v)) Pr (zip ST T) ->
+                     P cs ct (p_recv p L Pr) (ltt_recv p (zip L (zip ST T))).
+  Hypothesis P_send  : forall cs ct p l e Pr S T, typ_expr cs e S -> P cs ct Pr T -> P cs ct (p_send p l e Pr) (ltt_send p [(l,(S,T))]).
   
-  Fixpoint typ_proc_ind_ref (em : fin) (cs : ctxS) (ct : ctxT) (p : process) (T : ltt) (a : typ_proc em cs ct p T) {struct a} : P em cs ct p T.
+  Fixpoint typ_proc_ind_ref (cs : ctxS) (ct : ctxT) (p : process) (T : ltt) (a : typ_proc cs ct p T) {struct a} : P cs ct p T.
   Proof.
     refine (match a with
-      | tc_inact e s t Hs Ht => P_inact e s t Hs Ht
-      | tc_var e s t s1 t1 Hs Ht Hsl => P_var e s t s1 t1 Hs Ht Hsl
-      | tc_mu e sc tc x pr t t' Ht Hst => P_mu e sc tc x pr t t' (typ_proc_ind_ref e sc (extendT tc x t) pr t Ht) Hst
-      | tc_ite e sc tc ex p1 p2 t He Hp1 Hp2 => P_ite e sc tc ex p1 p2 t He (typ_proc_ind_ref e sc tc p1 t Hp1) (typ_proc_ind_ref e sc tc p2 t Hp2)
-      | tc_sub e sc tc pr t t' Ht Hst => P_sub e sc tc pr t t' (typ_proc_ind_ref e sc tc pr t Ht) Hst
-      | tc_recv e sc st p L ST Pr Tr HL HST HP HsL Hm => P_recv e sc st p L ST Pr Tr HL HST HP HsL _
-      | tc_send e sc tc p l ex Pr Sr Tr He HT => P_send e sc tc p l ex Pr Sr Tr He (typ_proc_ind_ref e sc tc Pr Tr HT)
+      | tc_inact s t => P_inact s t 
+      | tc_var s t s1 t1 Hsl => P_var s t s1 t1 Hsl
+      | tc_mu sc tc pr t t' Ht Hst => P_mu sc tc pr t t' (typ_proc_ind_ref sc (Some t :: tc) pr t' Ht) Hst
+      | tc_ite sc tc ex p1 p2 t He Hp1 Hp2 => P_ite sc tc ex p1 p2 t He (typ_proc_ind_ref sc tc p1 t Hp1) (typ_proc_ind_ref sc tc p2 t Hp2)
+      | tc_sub sc tc pr t t' Ht Hst => P_sub sc tc pr t t' (typ_proc_ind_ref sc tc pr t Ht) Hst
+      | tc_recv sc st p L ST Pr Tr HL HST HP HsL Hm => P_recv sc st p L ST Pr Tr HL HST HP HsL _
+      | tc_send sc tc p l ex Pr Sr Tr He HT => P_send sc tc p l ex Pr Sr Tr He (typ_proc_ind_ref sc tc Pr Tr HT)
     end); try easy.
     revert Hm.
-    apply Forall2_mono. intros. apply (typ_proc_ind_ref (S e) (extendS sc e (fst y)) st x (snd y) H).
+    apply Forall2_mono. intros. apply (typ_proc_ind_ref (Some (fst y) :: sc) st x (snd y) H).
   Qed.
 
 End typ_proc_ind_ref.
