process/inversion.v
@@ -5,89 +5,39 @@ From mathcomp Require Import ssreflect.seq.
 Import ListNotations.
 From Paco Require Import paco.
 
-Lemma empty_nil: forall {A: Type} (l: list A),
-  0 = length l <-> l = [].
-Proof. intros A l.
-       case l; intros; easy.
-Qed.
-   
 
-Lemma zip_eq: forall {A B: Type} (l1 l3: list A) (l2 l4: list B),
-  length l1 = length l2 -> length l2 = length l3 -> length l3 = length l4 ->
-  (zip l1 l2) = (zip l3 l4) ->
-  l1 = l3 /\ l2 = l4.
-Proof. intros A B l1.
-       induction l1; intros.
-       - simpl in *.
-         rewrite <- H in H0.
-         rewrite <- H0 in H1.
-         rewrite empty_nil in H.
-         rewrite empty_nil in H0.
-         rewrite empty_nil in H1.
-         subst. easy.
-       - simpl in H.
-         case_eq l2; intros.
-         + subst. simpl in *. easy.
-         + subst. simpl in *.
-           case_eq l3; intros.
-           ++ subst. easy.
-           ++ case_eq l4; intros.
-              -- subst. easy.
-              -- subst. simpl in *.
-                 inversion H2. subst.
-                 inversion H.
-                 inversion H1.
-                 inversion H0.
-                 specialize(IHl1 l0 l l2 H4 H7 H5 H6).
-                 split. f_equal. easy.
-                 f_equal. easy.
-Qed.
-
-Lemma zip_len: forall {A B: Type} (l1: list A) (l2: list B),
-  length l1 = length l2 -> length l1 = length (zip l1 l2).
-Proof. intros A B l1.
-       induction l1; intros.
-       - simpl in H. rewrite empty_nil in H.
-         subst. simpl. easy.
-       - simpl in H. simpl.
-         case_eq l2; intros.
-         subst. easy.
-         subst. simpl in H.
-         inversion H.
-         simpl. f_equal.
-         apply IHl1. easy.
-Qed.
-
-(* Lemma remove_S : forall {a b : fin}, S a = S b -> a = b.
-Proof.
-  intros.
-  inversion H. easy.
-Qed.
- *)
-Lemma _a23_a: forall em p L Q P Gs Gt T, 
-  typ_proc em Gs Gt P T ->
+Lemma _a23_a: forall p L Q P Gs Gt T, 
+  typ_proc Gs Gt P T ->
   P = (p_recv p L Q) -> 
-  (exists T' S, length T' = length L -> length T' = length S -> length T' = length Q -> subtypeC (ltt_recv p (zip (zip L S) T')) T /\ SSortedNList L /\ 
-  List.Forall2 (fun u v => typ_proc (Datatypes.S em) (extendS Gs em (fst v)) Gt u (snd v)) Q (zip S T')).
+  (exists T' ST, length T' = length L /\ length T' = length ST /\ length T' = length Q /\ subtypeC (ltt_recv p (zip L (zip ST T'))) T /\ SSortedNList L /\ 
+  List.Forall2 (fun u v => typ_proc (Some (fst v) :: Gs) Gt u (snd v)) Q (zip ST T')).
 Proof. intros.
        induction H; intros; try easy.
        specialize(IHtyp_proc H0).
-       destruct IHtyp_proc as (q',IHtyp_proc).
-       destruct IHtyp_proc.
-       exists q'. exists x. intros. destruct H2; try easy.
-       destruct H6. split.
-       specialize(stTrans (ltt_recv p (zip (zip L x) q')) t t' H2 H1); intros.
+       destruct IHtyp_proc. destruct H2. destruct H2. destruct H3. destruct H4. destruct H5. destruct H6.
+       exists x. exists x0.
+       split; try easy. split; try easy. split; try easy. split.
+       specialize(stTrans (ltt_recv p (zip L (zip x0 x))) t t' H5 H1); intros.
        easy.
        split. easy. easy.
-       inversion H0. subst. exists T. exists ST. intros.       
-       split. easy. split. easy. easy.
+       inversion H0. subst. exists T. exists ST.   
+       specialize(eq_trans H1 H2); intros.
+       specialize(eq_trans H H5); intros.
+       split; try easy.     
 Qed.
 
+(* Lemma _a23_af : forall p L Q P Gs Gt T T' ST,
+  typ_proc Gs Gt P T ->
+    P = (p_recv p L Q) -> 
+    length T' = length L -> length T' = length ST -> length T' = length Q -> SSortedNList L -> 
+    List.Forall2 (fun u v => typ_proc (Some (fst v) :: Gs) Gt u (snd v)) Q (zip ST T')) -> 
+    subtypeC (ltt_recv p (zip L (zip ST T'))) T. *)
 
-Lemma _a23_b: forall em p l e Q P Gs Gt T, 
-  typ_proc em Gs Gt P T ->
-  P = (p_send p l e Q) -> exists S S' T', typ_expr Gs e S /\ typ_proc em Gs Gt Q T' /\ subsort S' S /\ subtypeC (ltt_send p [(l,S',T')]) T.
-Proof. intros em p l e Q P Gs Gt T H.
+
+Lemma _a23_b: forall p l e Q P Gs Gt T, 
+  typ_proc Gs Gt P T ->
+  P = (p_send p l e Q) -> exists S S' T', typ_expr Gs e S /\ typ_proc Gs Gt Q T' /\ subsort S' S /\ subtypeC (ltt_send p [(l,(S',T'))]) T.
+Proof. intros p l e Q P Gs Gt T H.
        induction H; intros; try easy.
        specialize(IHtyp_proc H1).
        destruct IHtyp_proc as (S,(S',(T',Ha))).
@@ -96,38 +46,46 @@ Proof. intros em p l e Q P Gs Gt T H.
        specialize(sc_sub cs e S S); intro HSS.
        apply HSS. easy. apply srefl. 
        split.
-       specialize(tc_sub em cs ct Q T' T'); intro HTS.
+       specialize(tc_sub cs ct Q T' T'); intro HTS.
        apply HTS. easy.
        apply stRefl. split. easy.
        destruct Ha as (Ha,(Hb,(Hc,Hd))).
-       specialize(stTrans (ltt_send p [(l, S', T')]) t t' Hd H0); intro HT.
+       specialize(stTrans (ltt_send p [(l, (S', T'))]) t t' Hd H0); intro HT.
        apply HT.
        exists S. exists S. exists T.
        inversion H1. subst.
        split. easy. split. easy.
-       split. apply srefl. 
-       specialize(sub_out (upaco2 subtype bot2)
-          p [l] [S] [S] [T] [T]
-        ); intros HHa.
-       simpl in HHa.
-       pfold.
-       apply HHa. easy. easy.
-       apply Forall_forall. simpl.
-       intros (s1, s2) Hs. destruct Hs.
-       inversion H2. subst. simpl. apply srefl.
-       easy.
-       apply Forall_forall. simpl.
-       intros (T1, T2) Hs. destruct Hs.
-       inversion H2. subst.
-       simpl. left. pfold.
-       specialize(stRefl T2); intro HT.
-       punfold HT. apply st_mon.
-       easy.
+       split. apply srefl.
+       apply stRefl. 
 Qed.
 
-Lemma _a23_c: forall P em e Q1 Q2 T Gs Gt,
-  typ_proc em Gs Gt P T ->
-  P = (p_ite e Q1 Q2) -> exists T1 T2, typ_proc em Gs Gt Q1 T1 /\ typ_proc em Gs Gt Q2 T2 /\ subtypeC T1 T /\ subtypeC T2 T /\ typ_expr Gs e sbool.
+Lemma _a23_bf: forall p l e Q P Gs Gt T, 
+  typ_proc Gs Gt P T ->
+  P = (p_send p l e Q) -> exists S T', typ_expr Gs e S /\ typ_proc Gs Gt Q T' /\  subtypeC (ltt_send p [(l,(S,T'))]) T.
+Proof.
+  intros. revert H0. induction H; intros; try easy.
+  specialize(IHtyp_proc H1); intros. destruct IHtyp_proc. destruct H2. destruct H2. destruct H3.
+  exists x. exists x0. split; try easy. split; try easy.
+  specialize(stTrans (ltt_send p [(l, (x, x0))]) t t' H4 H0); intros; try easy.
+  inversion H1. subst.
+  exists S. exists T. split; try easy. 
+Qed.
+(* 
+Lemma _a23_bs: forall p l e Q P Gs Gt T, 
+  typ_proc Gs Gt P T ->
+  P = (p_send p l e Q) -> forall S T', subtypeC (ltt_send p [(l,(S,T'))]) T -> 
+  typ_expr Gs e S /\ typ_proc Gs Gt Q T'.
+Proof.
+  intros. revert H0. induction H; intros; try easy.
+  specialize(IHtyp_proc H1); intros. 
+  specialize(stTrans (ltt_send p [(l, (S, T'))]) t t' IHtyp_proc H0); intros; try easy.
+  inversion H3. subst.
+  exists S. exists T. split; try easy. 
+Qed.
+ *)
+Lemma _a23_c: forall P e Q1 Q2 T Gs Gt,
+  typ_proc Gs Gt P T ->
+  P = (p_ite e Q1 Q2) -> exists T1 T2, typ_proc Gs Gt Q1 T1 /\ typ_proc Gs Gt Q2 T2 /\ subtypeC T1 T /\ subtypeC T2 T /\ typ_expr Gs e sbool.
 Proof. intros.
        induction H; intros; try easy.
        inversion H0.
@@ -139,7 +97,7 @@ Proof. intros.
        destruct IHtyp_proc as (T1,(T2,(Ha,(Hb,(Hc,Hd))))).
        exists T1. exists T2.
        split.
-       specialize(tc_sub em cs ct Q1 T1 T1); intro HTS.
+       specialize(tc_sub cs ct Q1 T1 T1); intro HTS.
        apply HTS. easy. apply stRefl. split. easy. split. 
        specialize(stTrans T1 t t' Hc H1); intro HT. easy.
        split. destruct Hd.
@@ -147,238 +105,41 @@ Proof. intros.
        destruct Hd. easy.
 Qed.
 
-Lemma _a23_d: forall P em x Q T'' Gs Gt,
-  typ_proc em Gs Gt P T'' ->
-  P = (p_rec x Q)   -> exists T T', (typ_proc em Gs (extendT Gt x T) Q T' /\ subtypeC T T' /\ subtypeC T' T'').
+Lemma _a23_d: forall P Q T'' Gs Gt,
+  typ_proc Gs Gt P T'' ->
+  P = (p_rec Q)   -> exists T T', (typ_proc Gs (Some T :: Gt) Q T' /\ subtypeC T T' /\ subtypeC T' T'').
 Proof. intros.
        induction H; intros; try easy.
        inversion H0. subst.
-       exists t. exists t. 
+       exists t. exists t'. 
        split. easy. split. easy. easy.
        
        specialize(IHtyp_proc H0).
        destruct IHtyp_proc. destruct H2. 
-       exists x0. exists x1. 
+       exists x. exists x0.
        destruct H2. destruct H3. 
        split. easy. split. easy. 
-       specialize(stTrans x1 t t' H4 H1); intros. easy.
+       specialize(stTrans x0 t t' H4 H1); intros. easy.
 Qed. 
-(* 
 
-Lemma helper_a23_e_1 : forall x X n l x0 ct t, (Some t = lookupT ct X) -> (leq_ctxT (extendT x0 X x) ct) -> ((X =? n)%nat = false)
-    -> subtypeC x t -> leq_ctxT (consT X x (consT n l x0)) (consT n l ct).
-Proof. 
-  unfold leq_ctxT at 2. unfold leq_tinctx_prop.
-  induction lookupT; intros; try easy.
-  
-  case_eq (Nat.eqb n0 X); intros; try easy.
-  specialize(natb_to_prop n0 X H3); intros. subst. simpl.
-  replace (X =? X)%nat with true.
-  replace (X =? n)%nat with false.
-  replace (lookupT ct X) with (Some t).
-  easy.
-  
-  simpl. 
-  replace (n0 =? X)%nat with false.
-  case_eq (Nat.eqb n0 n); intros; try easy.
-  unfold leq_ctxT in H0. unfold leq_tinctx_prop in H0.
-  specialize(H0 n0). simpl in H0.
-  replace (n0 =? X)%nat with false in H0. easy.
-  
-  case_eq (Nat.eqb n0 X); intros; try easy.
-  specialize(natb_to_prop n0 X H3); intros. subst. simpl.
-  replace (X =? X)%nat with true.
-  replace (X =? n)%nat with false.
-  replace (lookupT ct X) with (Some t).
-  easy.
-  
-  simpl. 
-  replace (n0 =? X)%nat with false.
-  case_eq (Nat.eqb n0 n); intros; try easy.
-  unfold leq_ctxT in H0. unfold leq_tinctx_prop in H0.
-  specialize(H0 n0). simpl in H0.
-  replace (n0 =? X)%nat with false in H0. easy.
-  
-  apply emptyT.
-  apply 0.
-  
-Qed. *)
 
-Lemma refl_eq_ctxT : forall m, consistent_ctxT m -> eq_ctxT m m.
-Proof.
-  intros. 
-  unfold eq_ctxT. intros.
-  split. easy. split. easy.
-  induction lookupT. easy. easy.
-Qed.
-
-Lemma band_destruct : forall (a b : bool), true = a -> true = b -> true = (a && b)%bool.
-Proof.
-  intros. destruct H0. replace a with true. easy.
-Qed.
-
-Lemma bnat_comm : forall a b, ((a =? b)%nat = (b =? a)%nat).
-Proof. 
-      intros.
-      specialize(Nat.eqb_eq a b); intros.
-      specialize(Nat.eqb_eq b a); intros.
-      specialize(Nat.eqb_neq a b); intros.
-      specialize(Nat.eqb_neq b a); intros.
-      case_eq (a =? b)%nat.
-      - intros.
-        destruct H. specialize(H H3). 
-        specialize(eq_sym H); intros.
-        destruct H0. specialize(H6 H5). 
-        replace (b =? a)%nat with true.
-        easy.
-      - intros. destruct H1. specialize(H1 H3); intros.
-        specialize(not_eq_sym H1); intros.
-        destruct H2. specialize(H6 H5); intros. easy.
-Qed.
-
-Lemma swap_eq_ctxT : forall m X Y T T', consistent_ctxT (consT X T (consT Y T' m)) -> eq_ctxT (consT X T (consT Y T' m)) (consT Y T' (consT X T m)).
-Proof.
-  intros.
-  unfold eq_ctxT. intros.
-  split. easy. split. 
-  assert(consistent_ctxT (consT Y T' (consT X T m))).
-  {
-    simpl in H.
-    simpl.
-    case_eq (Nat.eqb X Y); intros.
-    replace (X =? Y)%nat with true in H. destruct H. easy.
-    replace (X =? Y)%nat with false in H.
-    specialize(bnat_comm Y X); intros.
-    specialize(eq_trans H1 H0); intros. 
-    replace (Y =? X)%nat with false.
-    split. destruct H. destruct H3.
-    easy. destruct H. destruct H3. split. easy. easy.
-  }
-  easy.
-  simpl. simpl in H.
-  case_eq (Nat.eqb n X); intros. 
-  - case_eq (Nat.eqb n Y); intros; try easy.
-    specialize(Nat.eqb_eq n X); intros. destruct H2. specialize(H2 H0); intros.
-    specialize(Nat.eqb_eq n Y); intros. destruct H4. specialize(H4 H1); intros.
-    specialize(eq_sym H2); intros. specialize(eq_trans H6 H4); intros.
-    specialize(Nat.eqb_eq X Y); intros. destruct H8. specialize(H9 H7); intros.
-    replace (X =? Y)%nat with true in H. simpl in H. easy.
-  - case_eq (Nat.eqb n Y); intros. try easy.
-    easy.
-Qed.
-
-Lemma sym_eq_ctxT : forall m1 m2, eq_ctxT m1 m2 -> eq_ctxT m2 m1.
-Proof.
-  intros.
-  unfold eq_ctxT in *.
-  intros.
-  specialize(H n); intros.
-  destruct H. destruct H0.
-  split. easy. split. easy. easy.
-Qed.
-
-Lemma trans_eq_ctxT : forall m1 m2 m3, 
-      eq_ctxT m1 m2 -> eq_ctxT m2 m3 -> eq_ctxT m1 m3.
-Proof.
-  intros.
-  unfold eq_ctxT in *.
-  intros.
-  split. specialize(H n); intros. easy. split. specialize(H0 n); intros. easy.
-  specialize(H n); intros.
-  specialize(H0 n); intros. 
-  destruct H0. destruct H1. destruct H. destruct H3. 
-  specialize(eq_trans H4 H2); intros. easy.
-Qed.
-  
-Lemma cons_eq_ctxT_helper : forall m1 m2 n, eq_ctxT m1 m2 -> lookupT m1 n = None -> lookupT m2 n = None.
-Proof. 
-  intros.
-  unfold eq_ctxT in H. specialize(H n); intros.
-  destruct H. destruct H1.
-  specialize(eq_trans (eq_sym H2) H0); intros.
-  easy.
-Qed.
-
-Lemma cons_eq_ctxT : forall m1 m2 n T, eq_ctxT m1 m2 -> lookupT m1 n = None -> eq_ctxT (consT n T m1) (consT n T m2).
-Proof.
-  intros.
-  pose proof H as H1.
-  unfold eq_ctxT. intros.
-  specialize(H n0); intros. destruct H. destruct H2. 
-  split.
-  simpl. split. easy. easy.
-  split. simpl. split. 
-  specialize(cons_eq_ctxT_helper m1 m2 n H1 H0); intros.
-  easy. easy.
-  simpl. 
-  case_eq (n0 =? n)%nat; intros; try easy.
-Qed.
-
-Lemma _a23_e: forall P em X T Gs Gt,
-  typ_proc em Gs Gt P T ->
-  (P = (p_var X) -> exists T' G', eq_ctxT (extendT G' X T') Gt /\ subtypeC T' T).
+Lemma _a23_e: forall P X T Gs Gt,
+  typ_proc Gs Gt P T ->
+  (P = (p_var X) -> exists T', onth X Gt = Some T' /\ subtypeC T' T).
 Proof. intros.
        induction H; intros; try easy.
        inversion H0. subst.
+       exists t. split. easy. easy.
        
-       induction ct. simpl in H2. easy.
-       simpl in H2.
-       case_eq (Nat.eqb X n); intros.
-       replace (X =? n)%nat with true in H2. inversion H2.
-       simpl in H1. destruct H1.
-       specialize(IHct H4); intros.
-       unfold extendT in *.
-       exists l. exists ct. split; try easy.
-       specialize(natb_to_prop X n H3); intros. replace X with n. easy.
-       
-       replace (X =? n)%nat with false in H2.
-       simpl in H1. destruct H1. 
-       specialize(IHct H4 H2); intros.
-       destruct IHct. destruct H5.
-       exists x. exists (extendT x0 n l).
-       unfold extendT in *.
-       destruct H5.
-       specialize(sym_eq_ctxT (consT X x x0) ct H5); intros.
-       specialize(cons_eq_ctxT ct (consT X x x0) n l H7 H1); intros.
-       Compute (swap_eq_ctxT).
-       specialize(swap_eq_ctxT x0 X n x l); intros.
-       specialize(sym_eq_ctxT (consT n l ct) (consT n l (consT X x x0))); intros.
-       
-       simpl in H9. replace (X =? n)%nat with false in H9. 
-       assert(lookupT x0 X = None /\ lookupT x0 n = None /\ consistent_ctxT x0).
-       {
-         split; try easy. 
-         unfold eq_ctxT in H5. simpl in H5.
-         specialize(H5 n); intros. destruct H5. destruct H5.
-         easy. split.
-         
-         unfold eq_ctxT in H8. simpl in H8.
-         specialize(bnat_comm n X ); intros. specialize(eq_trans H11 H3); intros.
-         replace (n =? X)%nat with false in H8.
-         specialize(H8 n); intros. destruct H8. destruct H13. destruct H13. easy.
-         
-         unfold eq_ctxT in H5. specialize(H5 n); intros. simpl in H5.
-         destruct H5. destruct H5. easy.
-       }
-       specialize(H9 H11); intros.
-       specialize(sym_eq_ctxT (consT X x (consT n l x0)) (consT n l (consT X x x0)) H9); intros.
-       specialize(trans_eq_ctxT (consT n l ct) (consT n l (consT X x x0)) (consT X x (consT n l x0)) H8 H12); intros.
-       split. 
-       specialize(sym_eq_ctxT (consT n l ct) (consT X x (consT n l x0)) H13); intros.
-       easy. easy.
-       
-       specialize(IHtyp_proc H0); intros.
-       destruct IHtyp_proc. destruct H2.
-       exists x. exists x0. 
-       destruct H2. split.
-       easy.
-       specialize(stTrans x t t' H3 H1); intros.
-       easy.
+       specialize(IHtyp_proc H0); intros. destruct IHtyp_proc.
+       destruct H2.
+       exists x. split. easy.
+       specialize(stTrans x t t' H3 H1); intros; try easy.
 Qed.
        
 
-Lemma _a23_f: forall P em T Gs Gt,
-  typ_proc em Gs Gt P T ->
+Lemma _a23_f: forall P T Gs Gt,
+  typ_proc Gs Gt P T ->
   P = p_inact -> T = ltt_end.
 Proof. intros.
        induction H; intros; try easy.
