process/substitution_examples.v
@@ -1,0 +1,19 @@
+From mathcomp Require Import all_ssreflect.
+From SST Require Import aux.unscoped aux.expressions type.global tree.global tree.local process.processes. 
+Require Import List String Datatypes ZArith Relations Setoid Morphisms.
+Open Scope list_scope.
+From mathcomp Require Import ssreflect.seq.
+Import ListNotations.
+From Paco Require Import paco.
+Require Import Coq.Init.Datatypes.
+Require Import Coq.Arith.PeanoNat. 
+Require Import JMeq.
+
+Definition P := (p_rec (p_ite (e_var 0) (p_var 0) (p_var 1))).
+
+Example subst1 : substitutionP 0 0 0 P (p_ite (e_var 2) (p_rec (p_ite (e_var 1) (p_var 0) (p_var 1))) (p_var 0)) 
+                                       (p_ite (e_var 2) (p_rec (p_ite (e_var 1) (p_var 0) (p_rec (p_ite (e_var 0) (p_var 0) (p_var 2))))) P).
+Proof.
+  unfold P.
+  repeat (constructor; try easy).
+Qed.
